language_formal/spark2014_semantics/util.v
@@ -10,17 +10,6 @@ zhangzhi@ksu.edu
 *)
 
 
-Inductive Return (A:Type): Type :=
-    | Normal: A -> Return A
-    | Run_Time_Error: Return A
-    | Unterminated: Return A
-    | Abnormal: Return A.
-(* TODO: add stuff in error states *)
-Arguments Normal [A] a.
-Arguments Run_Time_Error {A}.
-Arguments Unterminated {A}.
-Arguments Abnormal {A}.
-
 
 (** * Customized Tactics *)
 
